ARM that only adds verifies

verified/ARMspartan.dfy
@@ -1,5 +1,24 @@
 include "ARMdef.dfy"
 
+//-----------------------------------------------------------------------------
+// Utilities 
+//-----------------------------------------------------------------------------
+function pow2_32():int { 0x1_0000_0000 }
+predicate isUInt32(i:int) { 0 <= i < pow2_32() }
+
+//-----------------------------------------------------------------------------
+// Sequence Utilities
+//-----------------------------------------------------------------------------
+function SeqLength<T>(s:seq<T>) : int { |s| }
+function SeqDrop<T>(s:seq<T>, tail:int) : seq<T> 
+    requires 0 <= tail <= |s|;                                           
+    { s[..tail] }
+function SeqAppendElt<T>(s:seq<T>, elt:T) : seq<T> { s + [elt] }
+function SeqBuild<T>(elt:T) : seq<T> { [elt] }
+
+//-----------------------------------------------------------------------------
+// Spartan Types
+//-----------------------------------------------------------------------------
 type sp_int = int
 type sp_bool = bool
 type sp_operand = operand 
@@ -7,10 +26,11 @@ type sp_cmp = obool
 type sp_code = code
 type sp_codes = codes
 type sp_state = state
-function sp_eval_op(s:state, o:operand):int requires ValidOperand(s, o); { OperandContents(s, o) }
 
-function pow2_32():int { 0x1_0000_0000 }
-predicate isUInt32(i:int) { 0 <= i < pow2_32() }
+//-----------------------------------------------------------------------------
+// Spartan-Verification Interface
+//-----------------------------------------------------------------------------
+function sp_eval_op(s:state, o:operand):int requires ValidOperand(s, o); { OperandContents(s, o) }
 
 function method sp_CNil():codes { CNil }
 function sp_cHead(b:codes):code requires b.sp_CCons? { b.hd }
@@ -38,6 +58,9 @@ function method sp_get_ifFalse(c:code):code requires c.IfElse? { c.ifFalse }
 function method sp_get_whileCond(c:code):obool requires c.While? { c.whileCond }
 function method sp_get_whileBody(c:code):code requires c.While? { c.whileBody }
 
+//-----------------------------------------------------------------------------
+// Stack
+//-----------------------------------------------------------------------------
 function method stack(slot:int):operand {  OVar(IdStackSlot(slot)) }
 function stackval(s:sp_state, o:operand):int requires ValidOperand(s, o); { sp_eval_op(s, o) }
 predicate NonEmptyStack(s:sp_state) { s.stack != [] }
@@ -45,8 +68,169 @@ predicate StackContains(s:sp_state, slot:int)
     requires NonEmptyStack(s);
     { stack(slot).x in s.stack[0].locals }
 
+//-----------------------------------------------------------------------------
+// Heap
+//-----------------------------------------------------------------------------
+predicate HeapOperand(o:operand) { o.OHeap? }
 
+//-----------------------------------------------------------------------------
+// Register Validity
+//-----------------------------------------------------------------------------
 predicate ValidRegisters(s:sp_state)
 {
 	forall i:int :: 0 <= i <= 15 ==> ValidOperand(s, var_r(i))
+}
+
+//-----------------------------------------------------------------------------
+// Instruction Generation
+//-----------------------------------------------------------------------------
+function method{:opaque} sp_code_Add(dst:operand, src1:operand,
+	src2:operand):code { Ins(Add(dst, src1, src2)) }
+//TODO: everything else!
+
+//-----------------------------------------------------------------------------
+// Instruction Lemmas
+//-----------------------------------------------------------------------------
+lemma sp_lemma_Add(s:state, r:state, ok:bool,
+	dst:operand, src1:operand, src2:operand)
+	requires ValidOperand(s,src1);
+	requires ValidOperand(s,src2);
+	requires ValidDestinationOperand(s, dst);
+	requires sp_eval(sp_code_Add(dst, src1, src2), s, r, ok);
+	requires 0 <= OperandContents(s, dst) < MaxVal();
+	requires 0 <= OperandContents(s, src1) < MaxVal();
+	requires 0 <= OperandContents(s, src2) < MaxVal();
+	requires 0 <= OperandContents(s, src1) + OperandContents(s, src2) < MaxVal();
+	ensures  evalUpdate(s, dst, OperandContents(s, src1) +
+		OperandContents(s, src2), r, ok);
+	ensures  ok;
+	ensures  0 <= OperandContents(r, dst) < MaxVal();
+{
+	reveal_sp_eval();
+	reveal_sp_code_Add();
+}
+//TODO: everything else!
+
+//-----------------------------------------------------------------------------
+// Control Flow Lemmas
+//-----------------------------------------------------------------------------
+
+lemma sp_lemma_empty(s:state, r:state, ok:bool)
+  requires sp_eval(Block(sp_CNil()), s, r, ok)
+  ensures  ok
+  ensures  r == s
+{
+  reveal_sp_eval();
+}
+
+lemma sp_lemma_block(b:codes, s0:state, r:state, ok:bool) returns(r1:state, ok1:bool, c0:code, b1:codes)
+  requires b.sp_CCons?
+  requires sp_eval(Block(b), s0, r, ok)
+  ensures  b == sp_CCons(c0, b1)
+  ensures  sp_eval(c0, s0, r1, ok1)
+  ensures  ok1 ==> sp_eval(Block(b1), r1, r, ok)
+{
+  reveal_sp_eval();
+  assert evalBlock(b, s0, r, ok);
+  r1, ok1 :| sp_eval(b.hd, s0, r1, ok1) && (if !ok1 then !ok else evalBlock(b.tl, r1, r, ok));
+  c0 := b.hd;
+  b1 := b.tl;
+}
+
+lemma sp_lemma_ifElse(ifb:obool, ct:code, cf:code, s:state, r:state, ok:bool) returns(cond:bool)
+  requires ValidOperand(s, ifb.o1);
+  requires ValidOperand(s, ifb.o2);
+  requires sp_eval(IfElse(ifb, ct, cf), s, r, ok)
+  ensures  cond == evalOBool(s, ifb)
+  ensures  (if cond then sp_eval(ct, s, r, ok) else sp_eval(cf, s, r, ok))
+{
+  reveal_sp_eval();
+  cond := evalOBool(s, ifb);
+}
+
+// HACK
+lemma unpack_eval_while(b:obool, c:code, s:state, r:state, ok:bool)
+  requires evalCode(While(b, c), s, r, ok)
+  ensures  exists n:nat :: evalWhile(b, c, n, s, r, ok)
+{
+}
+
+predicate{:opaque} evalWhileOpaque(b:obool, c:code, n:nat, s:state, r:state, ok:bool) { evalWhile(b, c, n, s, r, ok) }
+
+predicate sp_whileInv(b:obool, c:code, n:int, r1:state, ok1:bool, r2:state, ok2:bool)
+{
+  n >= 0 && ok1 && evalWhileOpaque(b, c, n, r1, r2, ok2)
+}
+
+lemma sp_lemma_while(b:obool, c:code, s:state, r:state, ok:bool) returns(n:nat, r':state, ok':bool)
+  requires ValidOperand(s, b.o1)
+  requires ValidOperand(s, b.o2)
+  requires sp_eval(While(b, c), s, r, ok)
+  ensures  evalWhileOpaque(b, c, n, s, r, ok)
+  ensures  ok'
+  ensures  r' == s
+{
+  reveal_sp_eval();
+  reveal_evalWhileOpaque();
+  unpack_eval_while(b, c, s, r, ok);
+  n :| evalWhile(b, c, n, s, r, ok);
+  ok' := true;
+  r' := s;
+}
+
+lemma sp_lemma_whileTrue(b:obool, c:code, n:nat, s:state, r:state, ok:bool) returns(r':state, ok':bool)
+  requires ValidOperand(s, b.o1)
+  requires ValidOperand(s, b.o2)
+  requires n > 0
+  requires evalWhileOpaque(b, c, n, s, r, ok)
+  ensures  evalOBool(s, b)
+  ensures  sp_eval(c, s, r', ok')
+  ensures  (if !ok' then !ok else evalWhileOpaque(b, c, n - 1, r', r, ok))
+{
+  reveal_sp_eval();
+  reveal_evalWhileOpaque();
+  r', ok' :| evalOBool(s, b) && evalCode(c, s, r', ok') && (if !ok' then !ok else evalWhile(b, c, n - 1, r', r, ok));
+}
+
+lemma sp_lemma_whileFalse(b:obool, c:code, s:state, r:state, ok:bool)
+  requires ValidOperand(s, b.o1)
+  requires ValidOperand(s, b.o2)
+  requires evalWhileOpaque(b, c, 0, s, r, ok)
+  ensures  !evalOBool(s, b)
+  ensures  ok
+  ensures  r == s
+{
+  reveal_sp_eval();
+  reveal_evalWhileOpaque();
+}
+
+function ConcatenateCodes(code1:codes, code2:codes) : codes
+{
+    if code1.CNil? then
+        code2
+    else
+        sp_CCons(code1.hd, ConcatenateCodes(code1.tl, code2))
+}
+
+lemma lemma_GetIntermediateStateBetweenCodeBlocks(s1:sp_state, s3:sp_state, code1:codes, code2:codes, codes1and2:codes, ok1and2:bool)
+    returns (s2:sp_state, ok:bool)
+    requires evalBlock(codes1and2, s1, s3, ok1and2);
+    requires ConcatenateCodes(code1, code2) == codes1and2;
+    ensures  evalBlock(code1, s1, s2, ok);
+    ensures  if ok then evalBlock(code2, s2, s3, ok1and2) else !ok1and2;
+    decreases code1;
+{
+    if code1.CNil? {
+        s2 := s1;
+        ok := true;
+        return;
+    }
+
+    var s_mid, ok_mid :| evalCode(codes1and2.hd, s1, s_mid, ok_mid) && (if !ok_mid then !ok1and2 else evalBlock(codes1and2.tl, s_mid, s3, ok1and2));
+    if ok_mid {
+        s2, ok := lemma_GetIntermediateStateBetweenCodeBlocks(s_mid, s3, code1.tl, code2, codes1and2.tl, ok1and2);
+    }
+    else {
+        ok := false;
+    }
 }
